\begin{example}[Superposition]
\vspace{-1em}
\begin{gather*}
S = \{ {}^{1:}\mf(\mh(x))\foEQ\mc \lor \mh(\mh(x))\foNEQ \ma, 
	{}^{2:}\mh(y)\foEQ y, 
	{}^{3:}\mf(\ma)\foNEQ \mc \}\qquad\\[0.5em]
\newcommand{\stepA}{
	\infer[ \alpha % (S_+)\ \{ y\mapsto x \}
	]{	\mf(x)\foEQ\mc \lor {\colNA\mh(\mh(x))\foNEQ \ma}
	}{	^{2:}\mh(y)\foEQ y
		& 
		^{1:}\mf(\boxed{\mh(x)})\foEQ\mc \lor {\colNA\mh(\mh(x))\foNEQ \ma}
	}
}
\newcommand{\stepB}{
	\infer[	\beta]
	{		{\colNA\mh(\mh(\ma))\foNEQ \ma} \lor \mc\foNEQ\mc
	}{		\stepA & ^{3:}\boxed{\mf(\ma)}\foNEQ \mc
	}
}
\newcommand{\stepC}{
	\infer[\{\}
	]{		\mh(\boxed{\mh(\ma)})\foNEQ \ma
	}{		\stepB
	}
}
\newcommand{\stepD}{
	\infer[\gamma
	]{	\boxed{\mh(\ma)}\foNEQ\ma
	}{	^{2:}\mh(y)\foEQ y\hspace{-3cm} & \stepC
	}
}
\newcommand{\stepE}{
	\infer[\gamma
	]{	\ma\foNEQ\ma
	}{	^{2:}\mh(y)\foEQ y & \stepD
	}
}
\newcommand{\stepF}{
	\infer[\{\}	%(f)
	]{	\emptyclause
	}{	\stepE
	}
}
\stepF
\end{gather*}
\center
$\alpha = \{ y\mapsto x \}$, 
$\beta=\{ x\mapsto\ma\}$, 
$\gamma=\{ y\mapsto\ma\}$ 
\end{example}